Micro_Rust_Parser_Experiment/Micro_Rust_Parser_Command.thy
@@ -31,38 +31,173 @@ ML\<open>
    ONLY `parse_source` touches the Isabelle_lex_yacc global refs, so only it is serialized; elaboration and
    check_term are pure w.r.t. those, and holding the lock across them would serialize the (slower)
    type-checking of every uRust command theory-wide. *)
-fun elab_urust lthy source : term =
+datatype checked_urust =
+  Checked_URust of
+    {term: term,
+     translation: URust_Translate.result}
+
+fun elab_urust_result lthy source =
   (case
       (Parser_Utils.with_parser_lock
         (fn () => URust.parse_source lthy source)
        handle ERROR message =>
          error (URust_Diagnostics.humanize_parse_error message)) of
-     SOME ast => Syntax.check_term lthy (URust_Translate.mk_closed lthy ast)
+     SOME ast =>
+       let
+         val translation =
+           URust_Translate.make_result lthy ast
+         val checked =
+           Syntax.check_term lthy
+             (URust_Translate.result_term translation)
+       in
+         Checked_URust
+           {term = checked,
+            translation = translation}
+       end
    | NONE => error ("urust_expr: empty expression" ^ Position.here (Input.pos_of source)))
 
+fun elab_urust lthy source =
+  let val Checked_URust {term, ...} =
+    elab_urust_result lthy source
+  in term end
+
 fun define_urust_result (binding, source) lthy =
-  Local_Theory.define
-    ((binding, NoSyn), ((Thm.def_binding binding, []), elab_urust lthy source)) lthy
+  let
+    val Checked_URust {term, translation} =
+      elab_urust_result lthy source
+    val (definition, lthy') =
+      Local_Theory.define
+        ((binding, NoSyn),
+          ((Thm.def_binding binding, []), term)) lthy
+  in ((definition, translation), lthy') end
 
 fun define_urust args lthy = snd (define_urust_result args lthy)
 
 fun old_frontend_source source = "\<lbrakk> " ^ Input.string_of source ^ " \<rbrakk>"
 
+val legacy_normalization_factor = 256
+
 fun define_urust_with_frontend_check (binding, new_source, old_frontend_source) lthy =
   let
-    val ((lhs, (_, def_thm)), lthy') =
+    val (((lhs, (_, def_thm)), translation), lthy') =
       define_urust_result (binding, new_source) lthy
+    val _ =
+      if URust_Translate.legacy_compatible translation then ()
+      else
+        let
+          val (message, pos) =
+            URust_Translate.compatibility_diagnostic translation
+        in
+          error
+            ("urust_expr_with_check: scalable matcher form is not available" ^
+              " to the legacy frontend: " ^ message ^
+              "; use `urust_expr` for the scalable definition" ^
+              Position.here pos)
+        end
     val old_frontend =
       Syntax.parse_term lthy' old_frontend_source
     val equality =
       Syntax.check_term lthy'
         (Const (\<^const_name>\<open>HOL.eq\<close>, dummyT) $ lhs $ old_frontend)
+    val checked_rhs =
+      Thm.term_of (Thm.rhs_of def_thm)
+    val checked_size = Term.size_of_term checked_rhs
+    val legacy_size = Term.size_of_term old_frontend
+    val normalization_limit =
+      legacy_normalization_factor * checked_size + 8192
+    val _ =
+      if legacy_size <= normalization_limit then ()
+      else
+        error
+          ("urust_expr_with_check: bounded legacy normalization size " ^
+            string_of_int legacy_size ^ " exceeds " ^
+            string_of_int normalization_limit ^
+            Position.here (Input.pos_of new_source))
     val conformance =
       Goal.prove lthy' [] [] (HOLogic.mk_Trueprop equality)
         (fn {context = ctxt, ...} =>
-          Local_Defs.unfold_tac ctxt
-            [def_thm, @{thm urust_admin_let_def}] THEN
-          resolve_tac ctxt [@{thm refl}] 1)
+          let
+            val matcher_definitions =
+              @{thms
+                urust_matcher_fail_def
+                urust_matcher_succeed_def
+                urust_matcher_choice_def
+                urust_matcher_map_def
+                urust_matcher_product_def
+                urust_matcher_test_def
+                urust_matcher_lift_def
+                urust_matcher_destructure_def
+                urust_matcher_run_def
+                urust_matcher_run_guarded_def
+                urust_matcher_run_value_def
+                urust_matcher_run_guarded_value_def}
+            val matcher_simps =
+              ctxt addsimps
+                (@{thms micro_rust_simps} @
+                 @{thms
+                   bind_literal_unit
+                   bind_literal_unit2
+                   evaluate_conjunction_literal
+                   evaluate_eq_literal
+                   evaluate_ge_literal
+                   evaluate_gt_literal
+                   evaluate_le_literal
+                   evaluate_lt_literal
+                   evaluate_pure_if})
+            val unfold_matchers =
+              Local_Defs.unfold_tac ctxt matcher_definitions
+            val semantic_simps =
+              matcher_simps addsimps
+                @{thms
+                  two_armed_conditional_def
+                  Core_Expression.bind.simps
+                  urust_eq_def
+                  bindlift2_def}
+            fun case_splits goal =
+              let
+                fun collect (Const (name, _)) splits =
+                      (case Ctr_Sugar.ctr_sugar_of_case ctxt name of
+                         SOME sugar =>
+                           insert Thm.eq_thm_prop (#split sugar) splits
+                       | NONE => splits)
+                  | collect _ splits = splits
+              in Term.fold_aterms collect goal [] end
+            fun case_congruences goal =
+              let
+                fun collect (Const (name, _)) congruences =
+                      (case Ctr_Sugar.ctr_sugar_of_case ctxt name of
+                         SOME sugar =>
+                           insert Thm.eq_thm_prop
+                             (#case_cong sugar) congruences
+                       | NONE => congruences)
+                  | collect _ congruences = congruences
+              in Term.fold_aterms collect goal [] end
+            fun simp_cases simps index =
+              SUBGOAL
+                (fn (goal, _) =>
+                  let
+                    val splits = case_splits goal
+                    val congruences = case_congruences goal
+                  in
+                    asm_full_simp_tac
+                      (simps
+                        |> fold Simplifier.add_cong congruences
+                        |> fold Splitter.add_split_bang splits)
+                      index
+                  end)
+                index
+            fun finish_matcher_goal index =
+              TRY
+                (resolve_tac ctxt [@{thm expression_eqI2}] index THEN
+                 force_tac semantic_simps index) THEN
+              TRY (force_tac matcher_simps index)
+          in
+            Local_Defs.unfold_tac ctxt [def_thm] THEN
+            (resolve_tac ctxt [@{thm refl}] 1 ORELSE
+              (unfold_matchers THEN
+                simp_cases matcher_simps 1 THEN
+                ALLGOALS finish_matcher_goal))
+          end)
     val (_, lthy'') =
       Local_Theory.note
         ((Binding.suffix_name "_conformance" binding, []), [conformance]) lthy'
